src/proofs/no_slashable_attestations/supporting_lemmas/fnc_invs_1_26.dfy
@@ -1405,21 +1405,21 @@ module Fnc_Invs_1_26
     ensures inv10_body(s')
     { }
 
-    lemma lemma_inv16_f_start_next_duty(process: DVCState, attestation_duty: AttestationDuty, process': DVCState)
+    lemma lemma_inv_no_queued_att_duty_if_latest_served_att_duty_is_none_f_start_next_duty(process: DVCState, attestation_duty: AttestationDuty, process': DVCState)
     requires f_start_next_duty.requires(process, attestation_duty)
     requires process' == f_start_next_duty(process, attestation_duty).state        
-    requires inv8_body(process) || inv16_body(process)
-    ensures inv16_body(process')
+    requires inv8_body(process) || inv_no_queued_att_duty_if_latest_served_att_duty_is_none_body(process)
+    ensures inv_no_queued_att_duty_if_latest_served_att_duty_is_none_body(process')
     { }  
 
-    lemma lemma_inv16_f_check_for_next_queued_duty(
+    lemma lemma_inv_no_queued_att_duty_if_latest_served_att_duty_is_none_f_check_for_next_queued_duty(
         process: DVCState,
         process': DVCState
     )
     requires f_check_for_next_queued_duty.requires(process)
     requires process' == f_check_for_next_queued_duty(process).state    
-    requires inv8_body(process) || inv16_body(process)
-    ensures inv16_body(process')
+    requires inv8_body(process) || inv_no_queued_att_duty_if_latest_served_att_duty_is_none_body(process)
+    ensures inv_no_queued_att_duty_if_latest_served_att_duty_is_none_body(process')
     decreases process.attestation_duties_queue
     {
         if  && process.attestation_duties_queue != [] 
@@ -1441,16 +1441,16 @@ module Fnc_Invs_1_26
                             new_attestation_slashing_db
                         )                        
                     );
-                    lemma_inv16_f_check_for_next_queued_duty(process_mod, process');
+                    lemma_inv_no_queued_att_duty_if_latest_served_att_duty_is_none_f_check_for_next_queued_duty(process_mod, process');
                 }
                 else
                 { 
                     var process_mod := process.(
                         attestation_duties_queue := process.attestation_duties_queue[1..]
                     );     
-                    assert inv8_body(process_mod) || inv16_body(process_mod);
+                    assert inv8_body(process_mod) || inv_no_queued_att_duty_if_latest_served_att_duty_is_none_body(process_mod);
 
-                    lemma_inv16_f_start_next_duty(process_mod, process.attestation_duties_queue[0], process');
+                    lemma_inv_no_queued_att_duty_if_latest_served_att_duty_is_none_f_start_next_duty(process_mod, process.attestation_duties_queue[0], process');
                 }
         }
         else
@@ -1459,7 +1459,7 @@ module Fnc_Invs_1_26
         }
     }
 
-    lemma lemma_inv16_f_serve_attestation_duty(
+    lemma lemma_inv_no_queued_att_duty_if_latest_served_att_duty_is_none_f_serve_attestation_duty(
         process: DVCState,
         attestation_duty: AttestationDuty,
         process': DVCState
@@ -1467,18 +1467,18 @@ module Fnc_Invs_1_26
     requires f_serve_attestation_duty.requires(process, attestation_duty)
     requires process' == f_serve_attestation_duty(process, attestation_duty).state
     requires inv8_body(process)  
-    requires inv16_body(process)
-    ensures inv16_body(process')
+    requires inv_no_queued_att_duty_if_latest_served_att_duty_is_none_body(process)
+    ensures inv_no_queued_att_duty_if_latest_served_att_duty_is_none_body(process')
     {
         var process_mod := process.(
                 attestation_duties_queue := process.attestation_duties_queue + [attestation_duty],
                 all_rcvd_duties := process.all_rcvd_duties + {attestation_duty}
             );        
         
-        lemma_inv16_f_check_for_next_queued_duty(process_mod, process');        
+        lemma_inv_no_queued_att_duty_if_latest_served_att_duty_is_none_f_check_for_next_queued_duty(process_mod, process');        
     } 
 
-    lemma lemma_inv16_f_att_consensus_decided(
+    lemma lemma_inv_no_queued_att_duty_if_latest_served_att_duty_is_none_f_att_consensus_decided(
         process: DVCState,
         id: Slot,
         decided_attestation_data: AttestationData, 
@@ -1486,8 +1486,8 @@ module Fnc_Invs_1_26
     )
     requires f_att_consensus_decided.requires(process, id, decided_attestation_data)
     requires process' == f_att_consensus_decided(process, id, decided_attestation_data).state     
-    requires inv16_body(process)
-    ensures inv16_body(process')
+    requires inv_no_queued_att_duty_if_latest_served_att_duty_is_none_body(process)
+    ensures inv_no_queued_att_duty_if_latest_served_att_duty_is_none_body(process')
     {
         
         if  || !process.current_attestation_duty.isPresent()
@@ -1520,36 +1520,36 @@ module Fnc_Invs_1_26
                 )
             );
 
-        assert inv16_body(process);
+        assert inv_no_queued_att_duty_if_latest_served_att_duty_is_none_body(process);
 
         var ret_check_for_next_queued_duty := f_check_for_next_queued_duty(process);
         
-        lemma_inv16_f_check_for_next_queued_duty(process, ret_check_for_next_queued_duty.state);
+        lemma_inv_no_queued_att_duty_if_latest_served_att_duty_is_none_f_check_for_next_queued_duty(process, ret_check_for_next_queued_duty.state);
 
         assert process' == ret_check_for_next_queued_duty.state;
         
     }  
 
-    lemma lemma_inv16_f_listen_for_attestation_shares(
+    lemma lemma_inv_no_queued_att_duty_if_latest_served_att_duty_is_none_f_listen_for_attestation_shares(
         process: DVCState,
         attestation_share: AttestationShare,
         process': DVCState
     )
     requires f_listen_for_attestation_shares.requires(process, attestation_share)
     requires process' == f_listen_for_attestation_shares(process, attestation_share).state
-    requires inv16_body(process)
-    ensures inv16_body(process')
+    requires inv_no_queued_att_duty_if_latest_served_att_duty_is_none_body(process)
+    ensures inv_no_queued_att_duty_if_latest_served_att_duty_is_none_body(process')
     {}
 
-    lemma lemma_inv16_f_listen_for_new_imported_blocks(
+    lemma lemma_inv_no_queued_att_duty_if_latest_served_att_duty_is_none_f_listen_for_new_imported_blocks(
         process: DVCState,
         block: BeaconBlock,
         process': DVCState
     )
     requires f_listen_for_new_imported_blocks.requires(process, block)
     requires process' == f_listen_for_new_imported_blocks(process, block).state    
-    requires inv16_body(process)
-    ensures inv16_body(process')
+    requires inv_no_queued_att_duty_if_latest_served_att_duty_is_none_body(process)
+    ensures inv_no_queued_att_duty_if_latest_served_att_duty_is_none_body(process')
     {
         var new_consensus_instances_already_decided := f_listen_for_new_imported_blocks_helper_1(process, block);
 
@@ -1569,7 +1569,7 @@ module Fnc_Invs_1_26
                     rcvd_attestation_shares := process.rcvd_attestation_shares - att_consensus_instances_already_decided.Keys                    
                 );    
 
-        assert inv16_body(process);
+        assert inv_no_queued_att_duty_if_latest_served_att_duty_is_none_body(process);
                     
 
         if process.current_attestation_duty.isPresent() && process.current_attestation_duty.safe_get().slot in att_consensus_instances_already_decided
@@ -1585,34 +1585,34 @@ module Fnc_Invs_1_26
                 )                
             );
             
-            assert inv16_body(process);
+            assert inv_no_queued_att_duty_if_latest_served_att_duty_is_none_body(process);
 
-            lemma_inv16_f_check_for_next_queued_duty(process, process');
+            lemma_inv_no_queued_att_duty_if_latest_served_att_duty_is_none_f_check_for_next_queued_duty(process, process');
         }
         else
         {   
-            assert inv16_body(process);
+            assert inv_no_queued_att_duty_if_latest_served_att_duty_is_none_body(process);
         }
     }  
 
-    lemma lemma_inv16_f_resend_attestation_share(
+    lemma lemma_inv_no_queued_att_duty_if_latest_served_att_duty_is_none_f_resend_attestation_share(
         process: DVCState,
         process': DVCState)
     requires f_resend_attestation_share.requires(process)
     requires process' == f_resend_attestation_share(process).state    
-    requires inv16_body(process)
-    ensures inv16_body(process')
+    requires inv_no_queued_att_duty_if_latest_served_att_duty_is_none_body(process)
+    ensures inv_no_queued_att_duty_if_latest_served_att_duty_is_none_body(process')
     { }       
          
-    lemma lemma_inv16_add_block_to_bn(
+    lemma lemma_inv_no_queued_att_duty_if_latest_served_att_duty_is_none_add_block_to_bn(
         s: DVCState,
         block: BeaconBlock,
         s': DVCState 
     )
     requires add_block_to_bn.requires(s, block)
     requires s' == add_block_to_bn(s, block)
-    requires inv16_body(s)
-    ensures inv16_body(s')
+    requires inv_no_queued_att_duty_if_latest_served_att_duty_is_none_body(s)
+    ensures inv_no_queued_att_duty_if_latest_served_att_duty_is_none_body(s')
     { }
 
     lemma lemma_inv_strictly_increasing_queue_of_att_duties_f_start_next_duty(process: DVCState, attestation_duty: AttestationDuty, process': DVCState)
